txn-data-consistency/Serializable_2PC_2PL.thy
@@ -21,7 +21,7 @@ record cl_conf =
 record 'v svr_conf =
   svr_state :: "txid0 \<Rightarrow> state_svr"
   svr_vl :: "'v v_list"
-  svr_key_fp :: "txid0 \<Rightarrow> 'v key_fp"
+  svr_fp :: "txid0 \<Rightarrow> 'v key_fp"
 
 \<comment>\<open>System Global State: Clients and key Servers\<close>
 record 'v global_conf =
@@ -30,8 +30,8 @@ record 'v global_conf =
 
 \<comment> \<open>Translator functions\<close>
 
-abbreviation get_txn_cl :: "cl_id \<Rightarrow> 'v global_conf \<Rightarrow> txid0" where
-  "get_txn_cl cl s \<equiv> Tn_cl (cl_sn (cls s cl)) cl"
+abbreviation get_txn :: "cl_id \<Rightarrow> 'v global_conf \<Rightarrow> txid0" where
+  "get_txn cl s \<equiv> Tn_cl (cl_sn (cls s cl)) cl"
 
 subsubsection \<open>Simulation function\<close>
 
@@ -63,8 +63,8 @@ definition update_kv_all_txn :: "(txid0 \<Rightarrow> state_cl) \<Rightarrow> (t
 
 definition kvs_of_gs :: "'v global_conf \<Rightarrow> 'v kv_store" where
   "kvs_of_gs gs = (\<lambda>k.
-   update_kv_all_txn (\<lambda>t. cl_state (cls gs (get_cl_txn t)))
-    (svr_state (svrs gs k)) (svr_key_fp (svrs gs k)) (svr_vl (svrs gs k)))"
+   update_kv_all_txn (\<lambda>t. cl_state (cls gs (get_cl t)))
+    (svr_state (svrs gs k)) (svr_fp (svrs gs k)) (svr_vl (svrs gs k)))"
 
 definition views_of_gs :: "'v global_conf \<Rightarrow> (cl_id \<Rightarrow> view)" where
   "views_of_gs gs = (\<lambda>cl. cl_view (cls gs cl))"
@@ -86,7 +86,7 @@ datatype 'v ev = Prepare key txid0 | RLock key 'v txid0 | WLock key 'v "'v optio
 
 definition svr_t'_unchanged where
   "svr_t'_unchanged t k svrss svrss' \<equiv> (\<forall>t'. t' \<noteq> t \<longrightarrow>
-     svr_key_fp (svrss' k) t' = svr_key_fp (svrss k) t' \<and>
+     svr_fp (svrss' k) t' = svr_fp (svrss k) t' \<and>
      svr_state (svrss' k) t' = svr_state (svrss k) t')"
 
 definition other_insts_unchanged where
@@ -104,93 +104,98 @@ lemmas cl_unchanged_defs = svr_cl_cl'_unchanged_def other_insts_unchanged_def
 lemmas unchanged_defs = svr_unchanged_defs svr_cl_cl'_unchanged_def
 
 definition tid_match :: "'v global_conf \<Rightarrow> txid0 \<Rightarrow> bool" where
-  "tid_match s t \<equiv> cl_sn (cls s (get_cl_txn t)) = get_sn_txn t"
+  "tid_match s t \<equiv> cl_sn (cls s (get_cl t)) = get_sn t"
 
 abbreviation svr_state_trans where
   "svr_state_trans s k s' t from_stat to_stat \<equiv>
       svr_state (svrs s k) t = from_stat
     \<and> svr_vl (svrs s' k) = svr_vl (svrs s k)
-    \<and> svr_key_fp (svrs s' k) = svr_key_fp (svrs s k)
+    \<and> svr_fp (svrs s' k) = svr_fp (svrs s k)
     \<and> svr_state (svrs s' k) t = to_stat
     \<and> cl_svr_k'_t'_unchanged k s s' t
     \<and> tid_match s t"
 
+abbreviation last_ver_v :: "'v v_list \<Rightarrow> 'v" where
+  "last_ver_v vl \<equiv> v_value (last_version vl (full_view vl))"
+
 abbreviation is_locked :: "state_svr \<Rightarrow> bool" where
   "is_locked svr_st \<equiv> svr_st \<in> {read_lock, write_lock, no_lock}"
+
+abbreviation not_locked :: "state_svr \<Rightarrow> bool" where
+  "not_locked svr_st \<equiv> svr_st \<notin> {write_lock, read_lock}"
 
 definition updated_kvs :: "'v global_conf \<Rightarrow> cl_id \<Rightarrow> 'v kv_store" where
   "updated_kvs s cl \<equiv> (\<lambda>k. update_kv_all_txn
     (\<lambda>t. cl_state (cls (s \<lparr> cls := (cls s)
-      (cl := cls s cl \<lparr> cl_state := cl_committed \<rparr> ) \<rparr>) (get_cl_txn t)))
-    (svr_state (svrs s k)) (svr_key_fp (svrs s k)) (svr_vl (svrs s k)))"
+      (cl := cls s cl \<lparr> cl_state := cl_committed \<rparr> ) \<rparr>) (get_cl t)))
+    (svr_state (svrs s k)) (svr_fp (svrs s k)) (svr_vl (svrs s k)))"
 
 definition prepare where
-  "prepare s k s' t \<equiv>
-    cl_state (cls s (get_cl_txn t)) = cl_prepared
+  "prepare k t s s' \<equiv>
+    cl_state (cls s (get_cl t)) = cl_prepared
     \<and> svr_state_trans s k s' t working prepared"
 
 definition acq_rd_lock where \<comment>\<open>Read Lock acquired\<close>
-  "acq_rd_lock s k v s' t \<equiv>
-    cl_state (cls s (get_cl_txn t)) = cl_prepared
+  "acq_rd_lock k v t s s' \<equiv>
+    cl_state (cls s (get_cl t)) = cl_prepared
     \<and> (\<forall>t'. svr_state (svrs s k) t' \<noteq> write_lock)
     \<and> svr_state (svrs s k) t = prepared
     \<and> svr_vl (svrs s' k) = svr_vl (svrs s k)
-    \<and> v = v_value (last_version (svr_vl (svrs s k)) (full_view (svr_vl (svrs s k))))
-    \<and> svr_key_fp (svrs s' k) t W = None
-    \<and> svr_key_fp (svrs s' k) t R = Some v
+    \<and> v = last_ver_v (svr_vl (svrs s k))
+    \<and> svr_fp (svrs s' k) t W = None
+    \<and> svr_fp (svrs s' k) t R = Some v
     \<and> svr_state (svrs s' k) t = read_lock
     \<and> cl_svr_k'_t'_unchanged k s s' t
     \<and> tid_match s t"
 
 definition acq_wr_lock where \<comment>\<open>Write Lock acquired\<close>
-  "acq_wr_lock s k v ov s' t \<equiv>
-    cl_state (cls s (get_cl_txn t)) = cl_prepared
-    \<and> (\<forall>t'. svr_state (svrs s k) t' \<notin> {write_lock, read_lock})
+  "acq_wr_lock k v ov t s s' \<equiv>
+    cl_state (cls s (get_cl t)) = cl_prepared
+    \<and> (\<forall>t'. not_locked (svr_state (svrs s k) t'))
     \<and> svr_state (svrs s k) t = prepared
     \<and> svr_vl (svrs s' k) = svr_vl (svrs s k)
-    \<and> (ov = None \<or>
-       ov = Some (v_value (last_version (svr_vl (svrs s k)) (full_view (svr_vl (svrs s k))))))
-    \<and> svr_key_fp (svrs s' k) t W = Some v
-    \<and> svr_key_fp (svrs s' k) t R = ov
+    \<and> ov \<in> {None, Some (last_ver_v (svr_vl (svrs s k)))}
+    \<and> svr_fp (svrs s' k) t W = Some v
+    \<and> svr_fp (svrs s' k) t R = ov
     \<and> svr_state (svrs s' k) t = write_lock
     \<and> cl_svr_k'_t'_unchanged k s s' t
     \<and> tid_match s t"
 
 definition acq_no_lock where \<comment>\<open>No Lock needed\<close>
-  "acq_no_lock s k s' t \<equiv>
-    cl_state (cls s (get_cl_txn t)) = cl_prepared
-    \<and> svr_key_fp (svrs s' k) t W = None
-    \<and> svr_key_fp (svrs s' k) t R = None
+  "acq_no_lock k t s s' \<equiv>
+    cl_state (cls s (get_cl t)) = cl_prepared
+    \<and> svr_fp (svrs s' k) t W = None
+    \<and> svr_fp (svrs s' k) t R = None
     \<and> svr_state_trans s k s' t prepared no_lock"
 
 definition nok where \<comment>\<open>Lock not available\<close>
-  "nok s k s' t \<equiv>
-    cl_state (cls s (get_cl_txn t)) = cl_prepared
+  "nok k t s s' \<equiv>
+    cl_state (cls s (get_cl t)) = cl_prepared
     \<and> svr_state_trans s k s' t prepared notokay"
 
 definition commit where
-  "commit s k s' t \<equiv>
+  "commit k t s s' \<equiv>
     is_locked (svr_state (svrs s k) t)
-    \<and> cl_state (cls s (get_cl_txn t)) = cl_committed
+    \<and> cl_state (cls s (get_cl t)) = cl_committed
     \<and> svr_vl (svrs s' k) =
-        update_kv_key t (svr_key_fp (svrs s k) t) (full_view (svr_vl (svrs s k))) (svr_vl (svrs s k))
+        update_kv_key t (svr_fp (svrs s k) t) (full_view (svr_vl (svrs s k))) (svr_vl (svrs s k))
     \<and> svr_state (svrs s' k) t = committed
-    \<and> svr_key_fp (svrs s' k) t = svr_key_fp (svrs s k) t
+    \<and> svr_fp (svrs s' k) t = svr_fp (svrs s k) t
     \<and> cl_svr_k'_t'_unchanged k s s' t
     \<and> tid_match s t"
 
 definition abort where \<comment>\<open>Locks released (aborted)\<close>
-  "abort s k s' t \<equiv>
+  "abort k t s s' \<equiv>
     svr_state (svrs s k) t \<in> {read_lock, write_lock, no_lock, notokay}
-    \<and> cl_state (cls s (get_cl_txn t)) = cl_aborted
+    \<and> cl_state (cls s (get_cl t)) = cl_aborted
     \<and> svr_vl (svrs s' k) = svr_vl (svrs s k)
     \<and> svr_state (svrs s' k) t = aborted
-    \<and> svr_key_fp (svrs s' k) t = svr_key_fp (svrs s k) t
+    \<and> svr_fp (svrs s' k) t = svr_fp (svrs s k) t
     \<and> cl_svr_k'_t'_unchanged k s s' t
     \<and> tid_match s t"
 
 definition user_commit where
-  "user_commit s s' cl \<equiv>
+  "user_commit cl s s' \<equiv>
     cl_state (cls s cl) = cl_init
     \<and> cl_state (cls s' cl) = cl_prepared
     \<and> cl_sn (cls s' cl) = cl_sn (cls s cl)
@@ -198,40 +203,40 @@ definition user_commit where
     \<and> svr_cl_cl'_unchanged cl s s'"
 
 definition cl_commit where
-  "cl_commit s s' cl sn u'' F \<equiv>
+  "cl_commit cl sn u'' F s s' \<equiv>
     sn = cl_sn (cls s cl) \<and>
     u'' = (\<lambda>k. full_view (kvs_of_gs s k)) \<and>
-    F = (\<lambda>k. svr_key_fp (svrs s k) (get_txn_cl cl s)) \<and>
+    F = (\<lambda>k. svr_fp (svrs s k) (get_txn cl s)) \<and>
     cl_state (cls s cl) = cl_prepared \<and>
-    (\<forall>k. is_locked (svr_state (svrs s k) (get_txn_cl cl s))) \<and>
+    (\<forall>k. is_locked (svr_state (svrs s k) (get_txn cl s))) \<and>
     cl_state (cls s' cl) = cl_committed \<and>
     cl_sn (cls s' cl) = cl_sn (cls s cl) \<and>
     cl_view (cls s' cl) = full_view o (updated_kvs s cl) \<and>
     svr_cl_cl'_unchanged cl s s'"
 
 definition cl_abort where
-  "cl_abort s s' cl \<equiv>
+  "cl_abort cl s s' \<equiv>
     cl_state (cls s cl) = cl_prepared
-    \<and> (\<exists>k. svr_state (svrs s k) (get_txn_cl cl s) = notokay)
-    \<and> (\<forall>k. svr_state (svrs s k) (get_txn_cl cl s) \<in> {read_lock, write_lock, no_lock, notokay})
+    \<and> (\<exists>k. svr_state (svrs s k) (get_txn cl s) = notokay)
+    \<and> (\<forall>k. svr_state (svrs s k) (get_txn cl s) \<in> {read_lock, write_lock, no_lock, notokay})
     \<and> cl_state (cls s' cl) = cl_aborted
     \<and> cl_sn (cls s' cl) = cl_sn (cls s cl)
     \<and> cl_view (cls s' cl) = cl_view (cls s cl)
     \<and> svr_cl_cl'_unchanged cl s s'"
 
 definition cl_ready_c where
-  "cl_ready_c s s' cl \<equiv>
+  "cl_ready_c cl s s' \<equiv>
     cl_state (cls s cl) = cl_committed
-    \<and> (\<forall>k. svr_state (svrs s k) (get_txn_cl cl s) = committed)
+    \<and> (\<forall>k. svr_state (svrs s k) (get_txn cl s) = committed)
     \<and> cl_state (cls s' cl) = cl_init
     \<and> cl_sn (cls s' cl) = Suc (cl_sn (cls s cl))
     \<and> cl_view (cls s' cl) = cl_view (cls s cl)
     \<and> svr_cl_cl'_unchanged cl s s'"
 
 definition cl_ready_a where
-  "cl_ready_a s s' cl \<equiv>
+  "cl_ready_a cl s s' \<equiv>
     cl_state (cls s cl) = cl_aborted
-    \<and> (\<forall>k. svr_state (svrs s k) (get_txn_cl cl s) = aborted)
+    \<and> (\<forall>k. svr_state (svrs s k) (get_txn cl s) = aborted)
     \<and> cl_state (cls s' cl) = cl_init
     \<and> cl_sn (cls s' cl) = Suc (cl_sn (cls s cl))
     \<and> cl_view (cls s' cl) = cl_view (cls s cl)
@@ -247,22 +252,22 @@ definition gs_init :: "'v global_conf" where
                  cl_view = view_init \<rparr>),
     svrs = (\<lambda>k. \<lparr> svr_state = (\<lambda>t. working),
                  svr_vl = [version_init],
-                 svr_key_fp = (\<lambda>t. Map.empty)\<rparr>)
+                 svr_fp = (\<lambda>t. Map.empty)\<rparr>)
   \<rparr>"
 
 fun gs_trans :: "'v global_conf \<Rightarrow> 'v ev \<Rightarrow> 'v global_conf \<Rightarrow> bool" where
-  "gs_trans s (Prepare k t)         s' \<longleftrightarrow> prepare s k s' t" |
-  "gs_trans s (RLock k v t)         s' \<longleftrightarrow> acq_rd_lock s k v s' t" |
-  "gs_trans s (WLock k v ov t)      s' \<longleftrightarrow> acq_wr_lock s k v ov s' t" |
-  "gs_trans s (NoLock k t)          s' \<longleftrightarrow> acq_no_lock s k s' t" |
-  "gs_trans s (NOK k t)             s' \<longleftrightarrow> nok s k s' t" |
-  "gs_trans s (Commit k t)          s' \<longleftrightarrow> commit s k s' t" |
-  "gs_trans s (Abort k t)           s' \<longleftrightarrow> abort s k s' t" |
-  "gs_trans s (User_Commit cl)      s' \<longleftrightarrow> user_commit s s' cl" |
-  "gs_trans s (Cl_Commit cl sn u F) s' \<longleftrightarrow> cl_commit s s' cl sn u F" |
-  "gs_trans s (Cl_Abort cl)         s' \<longleftrightarrow> cl_abort s s' cl" |
-  "gs_trans s (Cl_ReadyC cl)        s' \<longleftrightarrow> cl_ready_c s s' cl" |
-  "gs_trans s (Cl_ReadyA cl)        s' \<longleftrightarrow> cl_ready_a s s' cl" |
+  "gs_trans s (Prepare k t)         s' \<longleftrightarrow> prepare k t s s'" |
+  "gs_trans s (RLock k v t)         s' \<longleftrightarrow> acq_rd_lock k v t s s'" |
+  "gs_trans s (WLock k v ov t)      s' \<longleftrightarrow> acq_wr_lock k v ov t s s'" |
+  "gs_trans s (NoLock k t)          s' \<longleftrightarrow> acq_no_lock k t s s'" |
+  "gs_trans s (NOK k t)             s' \<longleftrightarrow> nok k t s s'" |
+  "gs_trans s (Commit k t)          s' \<longleftrightarrow> commit k t s s'" |
+  "gs_trans s (Abort k t)           s' \<longleftrightarrow> abort k t s s'" |
+  "gs_trans s (User_Commit cl)      s' \<longleftrightarrow> user_commit cl s s'" |
+  "gs_trans s (Cl_Commit cl sn u F) s' \<longleftrightarrow> cl_commit cl sn u F s s'" |
+  "gs_trans s (Cl_Abort cl)         s' \<longleftrightarrow> cl_abort cl s s'" |
+  "gs_trans s (Cl_ReadyC cl)        s' \<longleftrightarrow> cl_ready_c cl s s'" |
+  "gs_trans s (Cl_ReadyA cl)        s' \<longleftrightarrow> cl_ready_a cl s s'" |
   "gs_trans s Skip2                 s' \<longleftrightarrow> s' = s"
 
 definition tps :: "('v ev, 'v global_conf) ES" where
